\def\pathToRoot{../../}\input{\pathToRoot headers/uebungHeader}

\begin{document}

% Use Basis x or Talk x, where x is the number of the session
\uebunghead{Talk 6}{Special Constructions in Categories}
\author{Maximilian Wuttke}

\hint{Read the slides for the definitions of the six constructions}

\section{Products and Coproducts}

\begin{exercise}[Product is unique up-to isomorphism]
  Proof that for every category $\cat{A}$ all products are isomorphic. Thus we can speak of \emph{the} product.
\end{exercise}

\begin{answer}
  \begin{proof}
    Let $X, Y \in \cat{A}$ and $P$ be a product of $X$ and $Y$ together with $p_1 \from P \to X, p_2 \from P \to Y$
    and $P'$ be a product of $X$ and $Y$ together with $p'_1 \from P' \to X, p'_2 \from P' \to Y$.

    Lets reconcider the definition of the \emph{product}:
    For every object $A \in \cat{A}$ and arrows $f_1 \from A \to X, f_2 \from A \to Y$ we get that there exists a unique map
    $\bar{f} \from A \to P$, such that
    \[ \xymatrix{
        &A \ar[ldd]_{f_1} \ar@{.>}[d]|{\bar{f}\vphantom{\bar{\bar{f}}}}
        \ar[rdd]^{f_2}&       \\
                &P \ar[ld]^{p_1} \ar[rd]_{p_2}                  &       \\
        X       &                                               &Y
    } \]
    commutes.
    Now we can instanciate $A$ with $P'$, $f_1$ with $p_1$, $f_2$ with $p_2$. By analogous instanciations we get the commuting diagramm
    \[ \xymatrix{
      & P \ar@/_/[ldd]_{p_1} \ar@/^/[rdd]^{p_2} & \\
      & P \ar[ld]^{p_1} \ar@/_/@{.>}[dd]|{\bar{f}} \ar@{.>}[u]|{f} \ar[rd]_{p_2} & \\
      X & & Y \\
      & P' \ar[lu]_{p_1'} \ar@/_/@{.>}[uu]|{\tilde{f}} \ar@{.>}[d]|{f'} \ar[ru]^{p'_2} & \\
      & P' \ar@/^/[luu]^{p'_1} \ar@/_/[ruu]_{p'_2} &
    } \]
    for exactly one $f, f', \tilde{f}, \bar{f}$. With the inner triangles we get:
    \begin{alignat*}{2}
      p_1  \of \tilde{f} &= p'_1 &\qquad p_2  \of \tilde{f} &= p'_2 \\
      p'_1 \of \bar{f}   &= p_1  &       p'_2 \of \bar{f}   &= p_2
    \end{alignat*}
    By substitution we get
    \begin{alignat*}{2}
      p_1   \of (\tilde{f} \of \bar{f}) &= p_1  &\qquad p_2  \of (\tilde{f} \of \bar{f}) &= p_2 \\
      p'_1  \of (\bar{f} \of \tilde{f}) &= p'_1 &       p'_2 \of (\bar{f} \of \tilde{f}) &= p'_2
    \end{alignat*}
    With the outer triangles we get:
    \begin{alignat*}{5}
      p_1  &\;\of&&\; f  &= p_1  &\qquad p_2  &\;\of&\; f  &= p_2 \\
      p'_1 &\;\of&&\; f' &= p'_1 &\qquad p'_2 &\;\of&\; f' &= p'_2
    \end{alignat*}
    Note that $f$ and $f'$ are \emph{unique} and the first equations hold for $f = 1_P$ and $f = \tilde{f} \of \bar{f}$, thus $\tilde{f} \of \bar{f} = 1_P$.
    The second equations holds for $f' = 1_{P'}$ and for $f' = \bar{f} \of \tilde{f}$, thus $\bar{f} \of \tilde{f} = 1_{P'}$.
    Thus $P$ and $P'$ are isomorphic. \qedhere
  \end{proof}
\end{answer}

\hint{We will now assume that all the 6 constructions are unique up-to isomorphism.}

\begin{definition}{Arbitrary\ product}
  Let $\cat{A}$ be a category, $I$ a set, and $(X_i)_{i \in I}$ a family of objects of $\cat{A}$.
  A \demph{product} of $(X_i)_{i \in I}$ consists of an object $P$ and a family of maps
  $\Bigl(P \toby{p_i} X_i\Bigr)_{i \in I}$
  with the property that for all objects $A$ and families of maps
  $\Bigl(A \toby{f_i} X_i\Bigr)_{i \in I}$
  there exists a unique map $\bar{f}\from A \to P$ such that
  $\forall i \in I: p_i \of \bar{f} = f_i$.
\end{definition}

\begin{exercise}[Greatest lower bound]
  Define the \emph{greatest lower bound} for an family of objects in a poset and proof that it is the arbitrary product of the family when the poset is seen as a category.
\end{exercise}

\begin{answer}
  Let $(A, \le)$ be a poset concidered as a category and $I$ a set.
  A \demph{lower bound} of a family $(x_i)_{i\in I}$ is an element $a \in A$, s.\,t. $\forall i \in I: a \le x_i$.
  $z \in A$ is a \demph{greatest lower bound} of this family if $\forall a \in A: \text{$a$ is a lower bound} \Rightarrow a \le z$.

  Let $z$ be a greatest lower bound of the family $(x_i)_{i\in I}$. We show that $z$ is a product of $(x_i)_{i\in I}$.
  \begin{proof}
    We first have to define a family of maps $\Bigl(z \toby{p_i} x_i\Bigr)_{i \in I}$.
    This is trivial since we have $\forall i \in I: z \le x_i$.
    Now let $a \in A$ be and objects and let $\Bigl(a \toby{f_i} x_i\Bigr)_{i \in I}$ be a family of maps from $a$.
    The existing of this maps means that $a$ is a upper bound of $(x_i)_{i\in I}$.
    Now by definition of least upper bound, $a \le z$, thus we have a arrow $\bar{f} \from a \to z$.
    All arrows are unique, thus $\bar{f}$ is unique and the diagram commutes. \qedhere
  \end{proof}
\end{answer}

\begin{definition}{Arbitrary\ coproduct}
  Let $\cat{A}$ be a category, $I$ a set, and $(X_i)_{i \in I}$ a family of objects of $\cat{A}$.
  A \demph{coproduct} of $(X_i)_{i \in I}$ consists of an object $S$ and a family of maps
  $\Bigl(X_i \toby{p_i} S\Bigr)_{i \in I}$
  with the property that for all objects $A$ and families of maps
  $\Bigl(X_i \toby{f_i} A\Bigr)_{i \in I}$
  there exists a unique map $\bar{f}\from S \to A$ such that
  $\forall i \in I: \bar{f} \of p_i = f_i$.
\end{definition}

\begin{exercise}[Least upper bound]
  Define the \emph{least upper bound} for a class of objects in a poset and proof that it is the arbitrary binary coproduct of the poset seen as a category.
\end{exercise}

\begin{answer}
  Let $(A, \le)$ be a poset concidered as a category and $I$ a set.
  A \demph{upper bound} of a family $(x_i)_{i\in I}$ is an element $a \in A$, s.\,t. $\forall i \in I: x_i \le z$.
  $z \in A$ is a \demph{least upper bound} of this family if $\forall a \in A: \text{$a$ is a upper bound} \Rightarrow z \le a$.

  Let $z$ be a least upper bound of the family $(x_i)_{i\in I}$. We show that $z$ is a coproduct of $(x_i)_{i\in I}$.
  \begin{proof}
    We first have to define a family of maps $\Bigl(x_i \toby{p_i} z\Bigr)_{i \in I}$.
    This is trivial since we have $\forall i \in I: x_i \le a$.
    Now let $a \in A$ be and objects and let $\Bigl(x_i \toby{f_i} a\Bigr)_{i \in I}$ be a family of maps to $a$.
    The existing of this maps means that $a$ is a lower bound of $(x_i)_{i\in I}$.
    Now by definition of least lower bound, $z \le a$, thus we have a arrow $\bar{f} \from z \to a$.
    All arrows are unique, thus $\bar{f}$ is unique and the diagram commutes. \qedhere
  \end{proof}
\end{answer}

\begin{exercise}[Disjoint union]
  \begin{itemize}
    \item[(a)]For an index set $I$ and a family of sets $(X_i)_{i \in I}$, define the arbitrary disjoint union $\coprod_{i \in I}{X_i}$.
    \item[(b)]Show that this arbitrary disjoint union is indeed the arbitrary coproduct in $\Set$.
  \end{itemize}
\end{exercise}

\begin{answer}
  First let define the arbitrary disjoint union:
  \begin{definition}{Arbitrary disjoint union}
    Let $I$ be an index set and let $(x_i)_{i \in I}$ be a family of sets.
    We define the arbitrary disjoint union of $(x_i)_{i\in I}$:
    $$\coprod_{i \in I} {x_i} := \bigcup_{i \in I} \set{ (x, i) \;\big|\; i \in I \land x \in x_i}$$
  \end{definition}
  Now let $I$ be an index set and let $(x_i)_{i\in I}$ be a family of sets. We show that $\coprod_{i \in I} {x_i}$ is the coproduct of $(x_i)_{i\in I}$.
  \begin{proof}
    We first define the projection maps: $p_i(a) := (a, i)$.
    Now let $A$ be a set and $\Bigl(x_i \toby{f_i} A\Bigr)_{i \in I}$ be a family of functions to $A$.
    We define $\bar{f} : \coprod_{i \in I} {x_i} \to A$ with $\bar{f}(a, i) := f_i(a)$.
    We have to show that $\bar{f}$ is the only function such that
    $\forall i \in I: \bar{f} \of p_i = f_i$.
    Let $i \in I$ and we check $a \in x_i$. $\bar{f}(p_i(a)) = \bar{f}(a,i) = f_i(a)$.
    Now let $\tilde{f} : \coprod_{i \in I} {x_i} \to A$ be another function sucht that
    $\forall i \in I: \tilde{f} \of p_i = f_i$.
    Let $(a, i) \in \coprod_{i \in I} {x_i}$. $\bar{f}(a,i)= f_i(a) = \tilde{f}(p_i(a)) = \tilde{f}(a,i)$.\qedhere
  \end{proof}
\end{answer}

\begin{exercise}[Direct Sum of Vector Spaces]
  In the talk we have seen that the direct sum $V \oplus W$ of two vector spaces $V, W$ over a fixed field $K$ is the coproduct of $V$ and $W$.
  Show that it is also the product.
\end{exercise}

\begin{answer}
  \begin{proof}
    We first define the projection functions $p_1 \from V \oplus W \to V, p_2 \from V \oplus W \to W$:
    \begin{alignat*}{1}
      p_1(x,y) &:= x \\
      p_2(x,y) &:= y
    \end{alignat*}
    Now let $A$ be a vector space and $f_1 \from A \to V, f_2 \from A \to W$ be linear functions.
    We define $\bar{f}(a) := (f_1(a), f_(2))$. We clearly have
    \begin{alignat*}{2}
      p_1(\bar{f}(a)) &= p_1(f_1(a), f_2(a)) = f_1(a) \\
      p_2(\bar{f}(a)) &= p_2(f_1(a), f_2(a)) = f_2(a).
    \end{alignat*}
    Thus the diagramm
    \[ \xymatrix{
        & A \ar[ldd]_{f_1} \ar@{.>}[d]|{\bar{f}\vphantom{\bar{\bar{f}}}} \ar[rdd]^{f_2} & \\
        & {V \oplus W} \ar[ld]^{p_1} \ar[rd]_{p_2} & \\
        V & & W
    } \]
    commutes. Now we have to show that $\bar{f}$ is the only map such that the above diagramm commutes.
    Let $\tilde{f} \from A \to V \oplus W$ be a map such that $p_1 \of \tilde{f} = f_1 \land p_2 \of \tilde{f} = f_2$.
    \[
      \tilde{f}(a) = \bigl(p_1(\tilde{f}(a)), p_2(\tilde{f}(a))\bigr) = \bigl(p_1(\bar{f}(a)), p_2(\bar{f}(a))\bigr) = \bar{f}(a)\qedhere
    \]
  \end{proof}
\end{answer}

\section{Equalizer and Coequalizer}

\begin{definition}{Minus-Core of Linear Maps in Vector Spaces}
  Let $V, W$ be Vector Spaces over a field $K$. Let $s, t \from V \to W$ be linear functions.
  We define the linear function $s - t := \lambda v\in V. \; v(s) - t(s)$.
  Remember the definition $\forall g \from V \to W: core(g) := \set{ v \in V | g(v) = 0 }$.
  Now $core (s - t) = \set{v \in V | s(v) = t (v) }$.
\end{definition}

\begin{exercise}[Equalizer of Vector Spaces]
  Let
  $\xymatrix{
      X \ar@<.5ex>[r]^s \ar@<-.5ex>[r]_t & Y
  }$
  be a diagramm in $Vect_K$ for a field $K$. Show that $core(s-t)$ is the equalizer for this diagramm.
\end{exercise}

\begin{answer}
  \begin{proof}
    Let $i \from core(s-t) \to X$ be a inclusion function. Let
    $\xymatrix{
      A \ar[r]^f & X \ar@<.5ex>[r]^s \ar@<-.5ex>[r]_t & Y
    }$
    be a commuting diagramm. Note that $f A \subseteq core(s-t)$.
    Thus we can define $\bar{f} \from A \to core(s-t)$ with $\bar{f}(a) := f(a)$.
    We see that $\forall a \in A: i(\bar{f}(a))=\bar{f}(a)=f(a)$, thus $i \of \bar{f} = f$.
    Let $\tilde{f} \from A \to core(s-t)$ be another map such that $i \of \tilde{f} = f$.
    Now $\tilde{f}(a) = i(\tilde{f}(a)) = i(\bar{f}(a)) = \bar{f}(a)$.
  \end{proof}
\end{answer}

\begin{definition}{Reflexive,\ symmetric\ and transitive\ closure}
  Let $X$ be a arbitrary set and $R \subseteq X \times X$ a binary relation over $X$.
  We define $R_0 := R \cup \set{ (y, x) | (x, y) \in R} \cup \set{ (x, x) | x \in X}$,
  the the \emph{reflexive, symmetric closure} of R.
  Now we define inductively $\forall n \in \nat$:
  \[R_{n+1} := \set{(x_1, x_3) \in R \times R \; | \; \exists x_2 \in X, (x_1, x_2) \in R_n \land (x_2, x_3) \in R_n}.\]
  Now $S := \bigcup_{n \in \nat}{R_n}$ is the reflexive, symmetric and transitive closure of $R$.
\end{definition}

\begin{exercise}[Coequalizer of sets]
  In this exercise we will first define \emph{reflexive symmetric transitive closures} and will define the coequalizer of $\Set$.
  \begin{itemize}
    \item[(a)]First we will show that the reflexive, symmetric and transitive closure of a relation $R$ is the \emph{least} equivalence relation containing $R$.
      Let $R$ be a relation over a set $X$ and $S$ be the reflexive, symmetric and transitive closure of $R$. Show following lemmas:
      \begin{itemize}
        \item[(i)]Show $\forall n\in\nat: R_n$ and $S$ are reflexive and symmetric.
        \item[(ii)]Show $\forall n\in\nat: R \subseteq R_n$ and $R \subseteq S$.
        \item[(iii)]Show that $R_n$ is \emph{monotone}, i.\,e. $\forall n,m\in\nat: n\le m \Rightarrow R_n \subseteq R_m$.
        \item[(iv)]Now show that $S$ is transitive.
          \begin{hint}
            Let $m\in\nat$. Show $\forall x_1, x_2, x_3: (x_1, x_2) \in S \Rightarrow (x_2, x_3) \in R_m \Rightarrow (x_1, x_3) \in S$ via $\nat$-induction.
          \end{hint}
        \item[(v)]Now show that $R$ is the \emph{least} equivalence relation containing $R$, i.\,e.
          $$\forall R': \text{$R'$ is a equivalence relation} \land R \subseteq R' \Rightarrow S \subseteq R'.$$
      \end{itemize}
    \item[(b)]Now we will define the coequalizer of $\Set$.
      Let $X, Y \in \Set, s, t \from X \to Y$.
      We make the following definitions:
      \begin{alignat*}{2}
        R    &:=& \set{(s(a), t(a)) | a\in Y} \\
        \sim &:=& \text{reflexive, symmetric and transitive closure of $R$} \\
        C    &:=& Y / \sim
      \end{alignat*}
      Note that $[y] := \set{ y' \in Y | (y, y') \in \sim}$ is the equivalence class of $y$ and $Y / \sim := \set{ [y] | y \in Y}$ is the set of all equivalence classes of $\sim$.
      Also note that no equivalence class can be empty and for $[y]$ we call $y$ a representant of this class.
      We define $i \from Y \to E$ with $i(y) := [y]$.
      \begin{itemize}
        \item[(i)]Show that the following diagramm commutes:
          $\xymatrix{
            X \ar@<.5ex>[r]^s \ar@<-.5ex>[r]_t & Y \ar[r]^i & C
          }$
        \item[(ii)]Let
          $\xymatrix{
            X \ar@<.5ex>[r]^s \ar@<-.5ex>[r]_t & Y \ar[r]^f & A
          }$
          be a cummutative diagramm. Show that $f$ respects equivalence, i.\,e. $\forall (y_1, y_2) \in \sim: f(y_1) = f(y_2)$.
          \begin{hint}
            ``Destruct'' $(y_1, y_2) \in \sim$ and do a $\nat$-induction.
          \end{hint}
        \item[(iii)]Now define $\bar{f} \from C \to A$, such that the following diagramm commutes and show that there can only be one:
          \[ \xymatrix{
            & & A  \\
            X \ar@<.5ex>[r]^s \ar@<-.5ex>[r]_t & Y \ar[ru]^f \ar[rd]_i \\
            & & C \ar@{.>}[uu]|{\bar{f}}
          } \]
        \item[(iv)]Show that the fork
          $\xymatrix{
            X \ar@<.5ex>[r]^s \ar@<-.5ex>[r]_t & Y \ar[r]^i & C
          }$
          is the coequalizer of
          $\xymatrix{
            X \ar@<.5ex>[r]^s \ar@<-.5ex>[r]_t & Y
          }$.
      \end{itemize}
  \end{itemize}
\end{exercise}

\begin{answer}
  \begin{itemize}
    \item[(a)]
      \begin{itemize}
        \item[(i)]
          \begin{proof}
            To show that $S$ is symmetric and reflexive, we choose $n := 0$. $R_0$ is by construction symmetric and reflexive.
            We will show symmetrie and reflexivity of $S_n$ seperately.
            \begin{itemize}
              \item[\emph{Reflexivity:}]
                Let $x \in X$. We show $\forall n\in\nat: (x, x) \in R_n$ by induction on $n\in\nat$.
                \begin{itemize}
                  \item[$n=0$:]
                    $R_0$ is by construction reflexive.
                  \item[$n \rightarrow n+1$:]
                    We know $(x, x) \in R_n$ by the inductive hypositive and show $(x, x) \in R_{n+1}$. By applying the definition of $R_{n+1}$
                    it is enough tow show $(x, x) \in R_n \land (x, x) \in R_n$ that is true with the inductive hypositive.
                \end{itemize}
                \item[\emph{Symmetrie:}]
                We show $\forall n\in\nat: \forall x_1,x_2 \in X: (x_1, x_2) \in R \Rightarrow (x_2, x_1) \in R$ by induction on $n\in\nat$.
                \begin{itemize}
                  \item[$n=0$:]
                    $R_0$ is by construction symmetric.
                  \item[$n \rightarrow n+1$:]
                    We know $\forall x_1,x_2 \in X: (x_1, x_2) \in R_{n} \Rightarrow (x_2, x_1) \in R$ by the inductive hypositive and have to show
                    $\forall x_1, x_2 \in X: (x_1, x_2) \in R_{n+1} \Rightarrow (x_2, x_1) \in R_{n+1}$.
                    Let $x_1, x_2 \in X$ with $(x_1, x_2) \in R_{n+1}$. By unfolding the definition of $R_{n+1}$ we get a $x$ with
                    $(x_1, x) \in R_n \land (x, x_2) \in R_n$ and have to show $(x_2, x_1) \in R_{n+1}$.
                    We apply the definition of $R_{n+1}$ and show $(x_2, y) \in R_n \land (x, x_1) \in R_n$.
                    Applying the inductive hypositive we it is enough to show $(x, x_2) \in R_n \land (x_1, y) \in R_n$ that is true by assumption. \qedhere
                \end{itemize}
            \end{itemize}
          \end{proof} % (a) (i)

        \item[(ii)]
          \begin{proof}
            To show that $S$ contains $R$ we choose $n := 0$. $R_0$ contains $R$ by construction. \\
            We show $\forall n\in\nat: \forall x_1,x_2\in X: (x_1, x_2) \in R \Rightarrow (x_1, x_2) \in R_n$ by induction on $n\in\nat$.
            \begin{itemize}
              \item[$n=0$:]
                $R_0$ contains $R$ by construction.
              \item[$n \rightarrow n+1$:]
                We assume $\forall x_1, x_2 : X, (x_1, x_2) \in R \Rightarrow (x_1, x_2) \in R_n$ by the induction hypositive.
                Let $x_1, x_2 \in X$ and $(x_1, x_2) \in R$. We show $(x_1, x_2) \in R_{n+1}$.
                We apply the definition of $R_{n+1}$ and show $(x_1, x_1) \in R_n \land (x_1, x_2) \in R_n$.
                The first we know with (a)(i) and the second by assumption. \qedhere
            \end{itemize}
          \end{proof} % (a) (ii)

        \item[(iii)]
          \begin{proof}
            Let $m,n\in\nat$ and $x_1, x_2 \in X$. We show $n \le m \Rightarrow (x_1, x_2) \in R_n \Rightarrow (x_1, x_2) \in R_m$ by induction on $n\in\nat$.
            \begin{itemize}
              \item[$n=0$:]
                We have $n \le 0$ and thus $n = 0$ and $(x_1, x_2) \in R_0$. We have to show $(x_1, x_2) \in R_0$ that is true by assumption.
              \item[$n \rightarrow n+1$:]
                We know $n \le m+1$ and $(x_1, x_2) \in R_n$. By the induction hypositive we also know
                $n \le m \Rightarrow (x_1, x_2) \in R_n \Rightarrow (x_1, x_2) \in R_m$.
                We have to show $(x_1, x_2) \in R_{m+1}$. We have two cases:
                \begin{itemize}
                  \item[$n = m+1$:]
                    The goal follows with the assumption $(x_1, x_2) \in R_{n=m+1}$.
                  \item[$n \le m$:]
                    We show $(x_1, x_2) \in R_{m+1}$ by applying the definition of $R_{m+1}$ and have to show $(x_1, x_1) \in R_m \land (x_1, x_2) \in R_m$.
                    The first we know with (a)(i) and the second by assumption. \qedhere
                \end{itemize}
            \end{itemize}
          \end{proof} % (a) (iii)

        \item[(iv)]
          \begin{proof}
          % TODO
          \end{proof} % (a) (iv)

        \item[(v)]
          \begin{proof}
          % TODO
          \end{proof} % (a) (iv)

      \end{itemize}

      % TODO Do we need part (a) at all?
    \item[(b)]
      \begin{itemize}
        \item[(i)]
          \begin{proof}
            Let $x \in X$. We have $i(s(x)=[s(x)]$ and $i(t(x))=[t(x)]$. It remains to show that $[s(x)]=[t(x)]$. Therefore it is enough to show that $s(x) \sim t(x)$.
            This is true since $\sim$ contains $R$ and $(s(x), t(x)) \in R$ by the construction of $R$.
          \end{proof} % (b) (i)

        \item[(ii)]
          \begin{proof}
            Let $(y_1, y_2) \in \sim$. Then be definition of $\sim$ we have a $n\in\nat$ such that $(y_1, y_2) \in R_n$.
            We show $\forall n\in\nat: \forall y_1,y_2 \in Y: (y_1, y_2) \in R_n \Rightarrow f (y_1) = f (y_2)$ by induction on $n\in\nat$.
            \begin{itemize}
              \item[$n=0$:]
                We have $(y_1, y_2) \in R_0$. This means $(y_1, y_2) \in R \lor (y_2, y_1) \in R \lor y_1 = y_2)$.
                We have to show $f(y_1) = f(y_2)$. Case analysis.
                \begin{itemize}
                  \item[1.] $(y_1,y_2) \in R$. Then we have $y_1 = s(a) \land y_2 = t(t)$ for some $a \in X$. $f (s (a)) = f (t (a))$ holds since $f$ commutes.
                  \item[2.] $(y_1,y_2) \in R$. Then we have $y_2 = s(a) \land y_1 = t(t)$ for some $a \in X$. $f (t (a)) = f (s (a))$ holds since $f$ commutes.
                  \item[3.] $y_1=y_2$. Then we have $f(y_1) = f(y_2)$.
                \end{itemize}
              \item[$n \rightarrow n+1$:]
                We have $(y_1, y_2) \in R_{n+1}$. Therefore we have a $y$ such that $(y_1, y) \in R_n \land (y, y_2) \in R_n$.
                With the inductive hypositive we know $\forall y_1, y_2 \in Y: (y_1, y_2) \in R_n \Rightarrow f (y_1) = f (y_2)$.
                By instanciating the inductive hypositive we know $f (y_1) = f (y) \land f (y) = f (y_2)$.
                Thus we get $f (y_1) = f (y_2)$ \qedhere
            \end{itemize}
          \end{proof} % (b) (ii)

        \item[(iii)]
          \newcommand{\choice}[1]{\set{#1}}
          We have to assume the axiom of choice. Because every equivalence class is non-empty, we get a function
          $\choice{ \_ } \from Y/\sim \to Y$ such that $\choice{ e } \sim x$ for every equivalence class $e$ and every object $x \in e$.

          We now define $\bar{f}(e) := f (\choice e)$.

          We have to show that the diagramm commutes. Note that commutativity of this diagramm is equivalent to $\bar{f} \of i =f$.
          Let $y \in Y$. We have to show $\bar{f}(\choice{i (y)}) = f(y)$. With (ii) it is enough to show $\choice{i (y)} \sim y$.
          This holds since $\choice{i (y)} = \choice{[y]} \sim y$, since $y \sim y$. \qedhere

          We finally have to show that $\bar{f}$ is the only function with that property.
          Let $\tilde{f} \from C \to A$ with $\tilde{f} \of i = f$. Let $c \in Y /\sim$.
          Then $\bar{f}(c) = f(\choice{c}) = \tilde{f}(i(\choice{c}) = \tilde{f}([\choice{c}]) = \tilde{f}(c)$.

        \item[(iv)]We know that there is only \emph{one} coequalizer (up-to isomorphism). By definition we have shown that our construction is \emph{a} coequalizer.
      \end{itemize}

  \end{itemize}
\end{answer}

\section{Pullbacks and Pushouts}

\begin{exercise}[Pullbacks\,vs.\,producs]
  Show that if $Z$ is terminal and
  \[ \xymatrix{
    P \ar[r]_{p_2} \ar[d]^{p_1} & Y \ar[d]_{t} \\
    X \ar[r]^s & Z
  } \]
  is the pullback square in $\cat{A}$ of $X, Y, Z, s, t$ then $X, Y$ is the product in $\cat{A}$.
\end{exercise}

\begin{exercise}[Pushouts\,vs.\,coproducs]
  Show that if $Z$ is initial and
  \[ \xymatrix{
    Z \ar[r]_s \ar[d]^t & X \ar[d]_{p_1} \\
    Y \ar[r]^{p_2} & P
  } \]
  is the pullback square in $\cat{A}$ of $X, Y, Z, s, t$, then $X + Y$ is the coproduct in $\cat{A}$.
\end{exercise}

\end{document}

%%% Local Variables:
%%% mode: latex
%%% TeX-master: t
%%% End:
% vim: ts=2 sts=2 sw=2 expandtab
